theories/stacked_borrows/examples/opt1.v
@@ -1,5 +1,5 @@
 From simuliris.simulation Require Import lifting.
-From simuliris.stacked_borrows Require Import primitive_laws proofmode adequacy.
+From simuliris.stacked_borrows Require Import primitive_laws proofmode adequacy examples.lib.
 From iris.prelude Require Import options.
 
 
@@ -35,7 +35,6 @@ Definition ex1_unopt : expr :=
     "v"
   .
 
-
 Definition ex1_opt : expr :=
     let: "x" := new_place (&mut int) "i" in
     retag_place "x" (RefPtr Mutable) int Default #[ScCallId 0];;
@@ -46,67 +45,20 @@ Definition ex1_opt : expr :=
     Free "x" ;;
     "v".
 
-(* TODO looks like this lemma should be put elsewhere? *)
-Lemma sim_new_place_local `{sborGS Σ} T v_t v_s π Φ :
-  ⌜length v_t = length v_s⌝ -∗
-  (∀ t l,
-    ⌜length v_s = tsize T⌝ -∗
-    ⌜length v_t = tsize T⌝ -∗
-    t $$ tk_local -∗
-    l ↦t∗[tk_local]{t} v_t -∗
-    l ↦s∗[tk_local]{t} v_s -∗
-    PlaceR l (Tagged t) T ⪯{π} PlaceR l (Tagged t) T [{ Φ }]) -∗
-  new_place T #v_t ⪯{π} new_place T #v_s [{ Φ }].
-Proof.
-  iIntros (Hlen_eq) "Hsim".
-  rewrite /new_place. sim_bind (Alloc _) (Alloc _).
-  iApply sim_alloc_local. iIntros (t l) "Htag Ht Hs". iApply sim_expr_base.
-  sim_pures.
-  source_bind (Write _ _).
-  (* gain knowledge about the length *)
-  iApply source_red_irred_unless; first done. iIntros (Hsize).
-  iApply (source_write_local with "Htag Hs"); [by rewrite replicate_length | done | ].
-  iIntros "Hs Htag". source_finish.
-
-  target_bind (Write _ _).
-  iApply (target_write_local with "Htag Ht"); [ by rewrite replicate_length | lia| ].
-  iIntros "Ht Htag". target_finish.
-
-  sim_pures. iApply ("Hsim" with "[//] [] Htag Ht Hs").
-  iPureIntro; lia.
-Qed.
-
-(* TODO: potentially have more modular lemmas for exploiting UB in order use the generic new_place lemma... *)
-
-(*Lemma let_irred1 ϕ P x e1 e2 σ : *)
-  (*IrredUnless ϕ P e1 σ →*)
-  (*IrredUnless ϕ P (Let x e1 e2) σ.*)
-(*Proof.*)
-  (*intros He1 Hnirred. *)
-
-(* TODO: maybe have nicer n-step irreducibility thing?
-  then we could use the above generic lemma for [new_place].
-   currently we don't use it since, in order to apply it, we'd need to use UB that happens during its execution...
-*)
 Lemma sim_opt1 `{sborGS Σ} :
   ⊢ log_rel ex1_opt ex1_unopt.
 Proof.
   log_rel.
   iIntros "%r_t %r_s #Hrel !# %π _".
-  sim_pures.
-  sim_apply (Alloc _) (Alloc _) sim_alloc_local "". iIntros (t l) "Htag Ht Hs".
-  iApply sim_expr_base. sim_pures.
-
-  source_bind (Write _ _).
-  destruct r_s as [v_s | ]; first last.
-  { iApply source_red_irred_unless; first done. by iIntros. }
-  (* gain knowledge about the length *)
-  iApply source_red_irred_unless; first done. iIntros (Hsize).
-  iApply (source_write_local with "Htag Hs"); [by rewrite replicate_length | done | ].
-  iIntros "Hs Htag". source_finish.
+  (* new place *)
+  simpl. source_bind (new_place _ _).
+  iApply source_red_reach_or_stuck; [ | done | ].
+  { intros; eapply new_place_reach_or_stuck. }
+  simpl. iIntros "(%v_s & -> & %Hsize)".
   iPoseProof (rrel_value_source with "Hrel") as (v_t) "(-> & #Hv)".
   iPoseProof (value_rel_length with "Hv") as "%Hlen".
-  target_apply (Write _ _) (target_write_local with "Htag Ht") "Ht Htag"; [ by rewrite replicate_length | lia| ].
+  iApply source_red_base. iModIntro. to_sim.
+  sim_apply (new_place _ _) (new_place _ _) sim_new_place_local "%t %l % % Htag Ht Hs"; first done.
   sim_pures.
 
   target_apply (Copy _) (target_copy_local with "Htag Ht") "Ht Htag"; first lia.
@@ -170,20 +122,15 @@ Lemma sim_opt1' `{sborGS Σ} :
 Proof.
   log_rel.
   iIntros "%r_t %r_s #Hrel !# %π _".
-  sim_pures.
-  sim_apply (Alloc _) (Alloc _) sim_alloc_local "". iIntros (t l) "Htag Ht Hs".
-  iApply sim_expr_base. sim_pures.
-
-  source_bind (Write _ _).
-  destruct r_s as [v_s | ]; first last.
-  { iApply source_red_irred_unless; first done. by iIntros. }
-  (* gain knowledge about the length *)
-  iApply source_red_irred_unless; first done. iIntros (Hsize).
-  iApply (source_write_local with "Htag Hs"); [by rewrite replicate_length | done | ].
-  iIntros "Hs Htag". source_finish.
+  (* new place *)
+  simpl. source_bind (new_place _ _).
+  iApply source_red_reach_or_stuck; [ | done | ].
+  { intros; eapply new_place_reach_or_stuck. }
+  simpl. iIntros "(%v_s & -> & %Hsize)".
   iPoseProof (rrel_value_source with "Hrel") as (v_t) "(-> & #Hv)".
   iPoseProof (value_rel_length with "Hv") as "%Hlen".
-  target_apply (Write _ _) (target_write_local with "Htag Ht") "Ht Htag"; [ by rewrite replicate_length | lia| ].
+  iApply source_red_base. iModIntro. to_sim.
+  sim_apply (new_place _ _) (new_place _ _) sim_new_place_local "%t %l % % Htag Ht Hs"; first done.
   sim_pures.
 
   target_apply (Copy _) (target_copy_local with "Htag Ht") "Ht Htag"; first lia.
