theories/stacked_borrows/examples/opt2.v
@@ -1,5 +1,5 @@
 From simuliris.simulation Require Import lifting.
-From simuliris.stacked_borrows Require Import proofmode lang.
+From simuliris.stacked_borrows Require Import proofmode lang adequacy examples.lib.
 From iris.prelude Require Import options.
 
 
@@ -57,19 +57,15 @@ Proof.
   sim_pures.
   sim_apply InitCall InitCall (sim_init_call) "". iIntros (c) "Hcall". iApply sim_expr_base. sim_pures.
 
-  sim_apply (Alloc _) (Alloc _) sim_alloc_local "". iIntros (t l) "Htag Ht Hs".
-  iApply sim_expr_base. sim_pures.
-
-  source_bind (Write _ _).
-  destruct r_s as [v_s | ]; first last.
-  { iApply source_red_irred_unless; first done. by iIntros. }
-  (* gain knowledge about the length *)
-  iApply source_red_irred_unless; first done. iIntros (Hsize).
-  iApply (source_write_local with "Htag Hs"); [by rewrite replicate_length | done | ].
-  iIntros "Hs Htag". source_finish.
+  (* new place *)
+  simpl. source_bind (new_place _ _).
+  iApply source_red_reach_or_stuck; [ | done | ].
+  { intros; rewrite subst_result; eapply new_place_reach_or_stuck. }
+  simpl. iIntros "(%v_s & -> & %Hsize)".
   iPoseProof (rrel_value_source with "Hrel") as (v_t) "(-> & #Hv)".
   iPoseProof (value_rel_length with "Hv") as "%Hlen".
-  target_apply (Write _ _) (target_write_local with "Htag Ht") "Ht Htag"; [ by rewrite replicate_length | lia| ].
+  iApply source_red_base. iModIntro. to_sim.
+  sim_apply (new_place _ _) (new_place _ _) sim_new_place_local "%t %l % % Htag Ht Hs"; first done.
   sim_pures.
 
   target_apply (Copy _) (target_copy_local with "Htag Ht") "Ht Htag"; first lia.
@@ -129,7 +125,6 @@ Qed.
 Definition ex2_unopt' : expr :=
     (* "x" is the local variable that stores the pointer value "i" *)
     let: "x" := new_place (& int) "i" in
-    (* (x, Tagged pid_x) ↦{tk_local} i *)
 
     (* retag_place reborrows the pointer value stored in "x" (which is "i"),
       then updates "x" with the new pointer value. A [Default] retag is
@@ -167,19 +162,15 @@ Proof.
   iIntros "%r_t %r_s #Hrel !# %π _".
   sim_pures.
 
-  sim_apply (Alloc _) (Alloc _) sim_alloc_local "". iIntros (t l) "Htag Ht Hs".
-  iApply sim_expr_base. sim_pures.
-
-  source_bind (Write _ _).
-  destruct r_s as [v_s | ]; first last.
-  { iApply source_red_irred_unless; first done. by iIntros. }
-  (* gain knowledge about the length *)
-  iApply source_red_irred_unless; first done. iIntros (Hsize).
-  iApply (source_write_local with "Htag Hs"); [by rewrite replicate_length | done | ].
-  iIntros "Hs Htag". source_finish.
+  (* new place *)
+  simpl. source_bind (new_place _ _).
+  iApply source_red_reach_or_stuck; [ | done | ].
+  { intros; eapply new_place_reach_or_stuck. }
+  simpl. iIntros "(%v_s & -> & %Hsize)".
   iPoseProof (rrel_value_source with "Hrel") as (v_t) "(-> & #Hv)".
   iPoseProof (value_rel_length with "Hv") as "%Hlen".
-  target_apply (Write _ _) (target_write_local with "Htag Ht") "Ht Htag"; [ by rewrite replicate_length | lia| ].
+  iApply source_red_base. iModIntro. to_sim.
+  sim_apply (new_place _ _) (new_place _ _) sim_new_place_local "%t %l % % Htag Ht Hs"; first done.
   sim_pures.
 
   target_apply (Copy _) (target_copy_local with "Htag Ht") "Ht Htag"; first lia.
@@ -221,3 +212,13 @@ Proof.
 
   sim_val. eauto.
 Qed.
+
+Section closed.
+  (** Obtain a closed proof of [ctx_rel]. *)
+  Lemma sim_opt2'_ctx : ctx_rel ex2_opt' ex2_unopt'.
+  Proof.
+    set Σ := #[sborΣ].
+    apply (log_rel_adequacy Σ)=>?.
+    apply sim_opt2'.
+  Qed.
+End closed.
