theories/stacked_borrows/examples/opt3_down.v
@@ -1,5 +1,5 @@
 From simuliris.simulation Require Import lifting.
-From simuliris.stacked_borrows Require Import proofmode lang.
+From simuliris.stacked_borrows Require Import proofmode lang adequacy examples.lib.
 From iris.prelude Require Import options.
 
 
@@ -51,19 +51,16 @@ Proof.
   iIntros "%r_t %r_s #Hrel !# %π _".
   sim_pures.
   sim_apply InitCall InitCall sim_init_call "". iIntros (c) "Hcall". iApply sim_expr_base. sim_pures.
-  sim_apply (Alloc _) (Alloc _) sim_alloc_local "". iIntros (t l) "Htag Ht Hs".
-  iApply sim_expr_base. sim_pures. simpl.
 
-  source_bind (Write _ _). simpl.
-  destruct r_s as [v_s | ]; first last.
-  { iApply source_red_irred_unless; first done. by iIntros. }
-  (* gain knowledge about the length *)
-  iApply source_red_irred_unless; first done. iIntros (Hsize). simpl.
-  iApply (source_write_local with "Htag Hs"); [ done | done | ].
-  iIntros "Hs Htag". source_finish.
+  (* new place *)
+  simpl. source_bind (new_place _ _).
+  iApply source_red_reach_or_stuck; [ | done | ].
+  { intros; rewrite subst_result; eapply new_place_reach_or_stuck. }
+  simpl. iIntros "(%v_s & -> & %Hsize)".
   iPoseProof (rrel_value_source with "Hrel") as (v_t) "(-> & #Hv)".
   iPoseProof (value_rel_length with "Hv") as "%Hlen".
-  target_apply (Write _ _) (target_write_local with "Htag Ht") "Ht Htag"; [ done | lia| ].
+  iApply source_red_base. iModIntro. to_sim.
+  sim_apply (new_place _ _) (new_place _ _) sim_new_place_local "%t %l % % Htag Ht Hs"; first done.
   sim_pures.
 
   target_apply (Copy _) (target_copy_local with "Htag Ht") "Ht Htag"; first lia.
@@ -112,7 +109,7 @@ Proof.
   sim_apply (Free _) (Free _) (sim_free_local with "Htag Ht Hs") "Htag"; [done..|]. sim_pures.
   iApply (sim_protected_unprotectN with "Hcall Htag_i Hi_t Hi_s []"); [ | apply lookup_insert | | ].
   { simpl. cbn in Hlen_t. intros i' Hi'. replace i' with O by lia. rewrite elem_of_union elem_of_singleton. eauto. }
-  { iApply big_sepL2_singleton. done. } 
+  { iApply big_sepL2_singleton. done. }
   iIntros "Hcall Htag_i Hi_t Hi_s".
   iApply (sim_remove_empty_calls t_i with "Hcall").
   { rewrite lookup_insert. done. }
@@ -123,5 +120,16 @@ Proof.
     apply map_eq. intros t'. rewrite delete_insert_delete delete_insert; done.
   }
   sim_pures.
-  iApply sim_expr_base. iExists r_t, r_s. eauto. 
+  iApply sim_expr_base. iExists r_t, r_s. eauto.
 Qed.
+
+
+Section closed.
+  (** Obtain a closed proof of [ctx_rel]. *)
+  Lemma sim_opt3_down_ctx : ctx_rel ex3_down_opt ex3_down_unopt.
+  Proof.
+    set Σ := #[sborΣ].
+    apply (log_rel_adequacy Σ)=>?.
+    apply sim_opt3_down.
+  Qed.
+End closed.
